merged trunk rev 889

acl2svn/branches/centaur/axioms.lisp
@@ -1431,6 +1431,20 @@
                    (intern (symbol-name x)
                            pack))))))
 
+(defmacro defun-*1* (fn &rest args)
+  `(defun ,(*1*-symbol fn) ,@args))
+
+(defparameter *defun-overrides* nil)
+
+(defmacro defun-overrides (name formals &rest rest)
+  `(progn (push ',name *defun-overrides*) ; see add-trip
+          (defun ,name ,formals
+            ,@(butlast rest 1)
+            (progn (chk-live-state-p ',name state)
+                   ,(car (last rest))))
+          (defun-*1* ,name ,formals
+            (,name ,@formals))))
+
 (defun our-import (syms pkg)
 
 ; We have seen a case in which Allegro CL 8.0 spent about 20% of the time in
@@ -7847,6 +7861,22 @@
   (implies (and (p1 x1) (p2 x2) ...)
            (q (mv-nth 'n (fn x1 x2 ...))))
 
+  ~i[Bounder Form 1 (or Form 2)]:
+  (implies (and (tau-intervalp i1)
+                ...
+                (or (equal (tau-interval-dom i1) 'dom1-1)
+                    ...)
+                ...
+                (in-tau-intervalp x1 i1)
+                ...)
+           (and (tau-intervalp (bounder-fn i1 ...))
+                (in-tau-intervalp ~i[target]
+                                  (bounder-fn i1 ...))))
+
+  where ~i[target] is
+  (fn x1 ... y1 ...)             in ~i[Form 1], and
+  (mv-nth 'n (fn x1 ... y1 ...)) in ~i[Form 2] 
+
   ~i[Big Switch]:
   (equal (fn . formals) body)
 
@@ -8081,6 +8111,38 @@
   ~ev[]
   This form of signature rule is just like form 1 except that it is useful for functions
   that return multiple-values and allows us to ``type-check'' their individual outputs.
+
+  ~bv[]
+  General Form: ~i[Bounder Forms 1 and 2]:
+  (implies (and (tau-intervalp i1)
+                ...
+                (or (equal (tau-interval-dom i1) 'dom1-1)
+                    ...)
+                ...
+                (in-tau-intervalp x1 i1)
+                ...)
+           (and (tau-intervalp (bounder-fn i1 ...))
+                (in-tau-intervalp ~i[target]
+                                  (bounder-fn i1 ...))))
+  ~ev[]
+  where ~i[target] is either ~c[(fn x1 ... y1 ...)] in ~i[Form 1] or
+  ~c[(mv-nth 'n (fn x1 ... y1 ...))] in ~i[Form 2].
+
+  This form is for advanced users only and the schema given above is
+  just a reminder of the general shape.  A ``bounder'' for a given function
+  symbol, ~c[fn], is a function symbol ~c[bounder-fn] that computes an interval
+  containing ~c[(fn x1 ... y1 ...)] (or its ~c[n]th component in the case of
+  Form 2 rules) from the intervals containing certain of the arguments of
+  ~c[fn].  The correctness theorem for a bounder function informs the tau
+  system that bounds for ~c[fn] are computed by ~c[bounder-fn] and sets up the
+  correspondence between the relevant arguments, ~c[xi], of ~c[fn] and the
+  intervals containing those arguments, ~c[ii] to which ~c[bounder-fn] is
+  applied.  When the tau system computes the tau for a call of ~c[fn], it
+  computes the tau of the relevant arguments and applies the bounder to the
+  intervals of those tau.  This provides a domain and upper and/or lower bounds
+  for the value of the term.  The tau system then further augments that with
+  signature rules.  ~l[bounders] for details on intervals, bounders, and
+  bounder correctness theorems.
 
   ~bv[]
   General Form: ~i[Big Switch]:
@@ -21265,8 +21327,8 @@
   ~c[defattach], by permitting use of ~c[:]~ilc[program] mode functions and the
   skipping of semantic checks.  Also permitted is ~c[:skip-checks nil] (the
   default) and ~c[:skip-checks :cycles], which turns off only the update of the
-  extended ancestor relation and hence the check for cycles in this relation;
-  see below.  We do not make any logical claims when the value of
+  extended ancestor relation (see below) and hence the check for cycles in this
+  relation; see below.  We do not make any logical claims when the value of
   ~c[:skip-checks] is non-~c[nil]; indeed, a trust tag is required in this
   case (~pl[defttag]).  Remark for those who use the experimental HONS
   extension (~pl[hons-and-memoization]): the interaction of memoization and
@@ -21350,9 +21412,16 @@
   in mind that evaluation with the attachment equations takes place in an
   extension of the logical theory of the session.  ACL2 guarantees that this
   so-called ``evaluation theory'' remains consistent, assuming that the absence
-  of ~ilc[defaxiom] ~il[events] from the user.  A deeper discussion of the
-  logical issues is available (but not intended to be read by most users) in a
-  comment in the ACL2 source code labeled ``Essay on Defattach.''
+  of ~ilc[defaxiom] ~il[events] from the user.  This guarantee is a consequence
+  of a more general guarantee: an ACL2 logical ~il[world] exists in
+  which (loosely speaking) the attachment equation for ~c[(defattach f g)], as
+  ~c[(defun f (...) (g ...))], takes the place of the original defining event
+  for ~c[f], for each ~c[defattach] event.  This more general guarantee holds
+  even if there are ~ilc[defaxiom] events, though as explained below, no
+  function symbol that syntactically supports a ~c[defaxiom] formula is allowed
+  to get an attachment.  A deeper discussion of the logical issues is
+  available (but not intended to be read by most users) in a long comment in
+  the ACL2 source code labeled ``Essay on Defattach.''
 
   ~bv[]
   Example Forms:
@@ -21530,15 +21599,14 @@
   practical perspective, there would be an infinite loop resulting from any
   call of ~c[f].
 
-  We consider a function symbol ~c[g] to be an ``extended ancestor of'' a
-  function symbol ~c[f] if either of the following two criteria is met: (a)
-  ~c[g] occurs in the formula that introduces ~c[f] (i.e., definition body or
-  constraint) and ~c[g] is introduced by an event different from (earlier than)
-  the event introducing ~c[f]; or (b) ~c[g] is attached to ~c[f].  For a
-  proposed ~c[defattach] event, we check that the resulting extended ancestor
-  relation has no cycles, where for condition (b) we include all attachment
-  pairs that would result, including those remaining from earlier ~c[defattach]
-  events.
+  We consider a function symbol ~c[g] to be an ``extended immediate ancestor
+  of'' a function symbol ~c[f] if either of the following two criteria is
+  met: (a) ~c[g] occurs in the formula that introduces ~c[f] (i.e., definition
+  body or constraint) and ~c[g] is introduced by an event different
+  from (earlier than) the event introducing ~c[f]; or (b) ~c[g] is attached to
+  ~c[f].  For a proposed ~c[defattach] event, we check that this relation has
+  no cycles, where for condition (b) we include all attachment pairs that would
+  result, including those remaining from earlier ~c[defattach] events.
 
   Of course, a special case is that no function symbol may be attached to
   itself.  Similarly, no function symbol may be attached to any of its
@@ -21608,6 +21676,44 @@
 
   ~c[Defattach] events are illegal inside any ~ilc[encapsulate] event with a
   non-empty ~il[signature] unless they are ~il[local] to the ~ilc[encapsulate].
+
+  We next discuss a restriction based on a notion of a function symbol
+  syntactically supporting an event.  Function symbol ~c[f] is ~em[ancestral]
+  in event ~c[E] if either ~c[f] occurs in ~c[E], or (recursively) ~c[f] occurs
+  in an event ~c[E'] that introduces some function symbol ~c[g] that is
+  ancestral in ~c[E].  We require that no function symbol ancestral in the
+  formula of a ~ilc[defaxiom] event may have an attachment.  Theoretical
+  reasons are discussed in comments in the ACL2 source code, but here we give a
+  little example showing the need for some such restriction: without it, we
+  show how to prove ~c[nil]!
+  ~bv[]
+  (defn g1 () 1)
+  (defn g2 () 2)
+  (defstub f1 () t)
+  (defstub f2 () t)
+  (defund p (x)
+    (declare (ignore x))
+    t)
+  (defevaluator evl evl-list
+    ((p x)))
+  (defaxiom f1-is-f2
+    (equal (f1) (f2)))
+  (defun meta-fn (x)
+    (cond ((equal (f1) (f2))
+           x)
+          (t *nil*)))
+  (defthm bad-meta-rule
+    (equal (evl x a)
+           (evl (meta-fn x) a))
+    :rule-classes ((:meta :trigger-fns (p))))
+  (defattach f1 g1)
+  (defattach f2 g2)
+  (defthm contradiction
+    nil
+    :hints ((\"Goal\" :use ((:instance (:theorem (not (p x)))
+                                     (x t)))))
+    :rule-classes nil)
+  ~ev[]
 
   To see all attachments: ~c[(all-attachments (w state))].  (Note that
   attachments introduced with a non-~c[nil] value of ~c[:skip-checks] will be
@@ -23454,7 +23560,7 @@
               (symbolp (cadr x))
               (null (cddr x)))
 
-; The cmulisp complier complains about unreachable code every (perhaps) time
+; The cmulisp compiler complains about unreachable code every (perhaps) time
 ; that f-get-global is called in which st is *the-live-state*.  The following
 ; optimization is included primarily in order to eliminate those warnings;
 ; the extra efficiency is pretty minor, though a nice side effect.
@@ -27193,11 +27299,9 @@
 ; Functions in this list should be executed only in raw Lisp, hence perhaps not
 ; in safe-mode.  See the case of 'program-only-er in ev-fncall-msg.
 
-; This list is used in defining state global 'program-fns-with-raw-code, whose
-; value has been expanded significantly (from the corresponding old state
-; global, 'built-in-program-mode-fns) in Version_3.4.  If errors are caused by
-; attempting to call some of these functions in safe-mode, consider adding such
-; functions to the list *oneify-primitives*.
+; This list is used in defining state global 'program-fns-with-raw-code.  If
+; errors are caused by attempting to call some of these functions in safe-mode,
+; consider adding such functions to the list *oneify-primitives*.
 
   '(relieve-hyp-synp ; *deep-gstack*
     apply-abbrevs-to-lambda-stack1 ; *nth-update-tracingp*
@@ -27227,7 +27331,6 @@
     dmr-start-fn ; dmr-start-fn-raw
     memo-exit ; *nu-memos*
     memo-key1 ; *nu-memos*
-    sys-call-status ; *last-sys-call-status*
     ev-fncall-meta ; *metafunction-context*
     ld-loop ; *ld-level*
     print-summary ; dmr-flush
@@ -27256,7 +27359,6 @@
     flpr ; print-flat-infix
     close-trace-file-fn ; *trace-output*
     ev-fncall-rec ; raw-ev-fncall
-    sys-call ; system-call
     ev-fncall ; live-state-p
     ld-fn0 ; *acl2-unwind-protect-stack*, etc.
     ld-fn  ; unwind-protect
@@ -27315,7 +27417,6 @@
     state-p1 ; LIVE-STATE-P
     aref2 ; aref, slow-array-warning
     aref1 ; aref, slow-array-warning
-    mfc-ancestors ; *metafunction-context*
     fgetprop ; EQ, GET, ...
     getenv$ ; GETENV$-RAW
     wormhole-eval ; *WORMHOLE-STATUS-ALIST*
@@ -27329,7 +27430,6 @@
     time-limit5-reached-p ; THROW
     fmt-to-comment-window ; *THE-LIVE-STATE*
     len ; len1
-    mfc-clause ; *metafunction-context*
     cpu-core-count ; CORE-COUNT-RAW
     nonnegative-integer-quotient ; floor
     check-print-base ; PRIN1-TO-STRING
@@ -27343,14 +27443,11 @@
     strip-cars ; strip-cars1
     plist-worldp ; *the-live-state* (huge performance penalty?)
     wormhole-p ; *WORMHOLEP*
-    mfc-type-alist ; *metafunction-context*
     may-need-slashes-fn ;*suspiciously-first-numeric-array* ...
     fmt-to-comment-window! ; *THE-LIVE-STATE*
     has-propsp ; EQ, GET, ...
     hard-error ; *HARD-ERROR-RETURNS-NILP*, FUNCALL, ...
     abort! p! ; THROW
-    mfc-rdepth ; *metafunction-context*
-    mfc-unify-subst ; *metafunction-context*
     flush-compress ; SETF [may be critical for correctness]
     alphorder ; [bad atoms]
     extend-world ; EXTEND-WORLD1
@@ -27399,7 +27496,6 @@
     good-bye-fn ; exit-lisp
     remove-eq remove-equal
     take
-    canonical-pathname
     file-write-date$
     print-call-history
     set-debugger-enable-fn ; lisp::*break-enable* and *debugger-hook*
@@ -27425,6 +27521,28 @@
     time-tracker-fn
     gc-verbose-fn
     set-absstobj-debug-fn
+    sys-call-status ; *last-sys-call-status*
+    sys-call ; system-call
+
+    canonical-pathname ; under dependent clause-processor
+
+; mfc functions
+
+    mfc-ancestors ; *metafunction-context*
+    mfc-clause ; *metafunction-context*
+    mfc-rdepth ; *metafunction-context*
+    mfc-type-alist ; *metafunction-context*
+    mfc-unify-subst ; *metafunction-context*
+    mfc-ap-fn ; under dependent clause-processor
+    mfc-ap-ttree ; under dependent clause-processor
+    mfc-relieve-hyp-fn ; under dependent clause-processor
+    mfc-relieve-hyp-ttree ; under dependent clause-processor
+    mfc-rw+-fn ; under dependent clause-processor
+    mfc-rw+-ttree ; under dependent clause-processor
+    mfc-rw-fn ; under dependent clause-processor
+    mfc-rw-ttree ; under dependent clause-processor
+    mfc-ts-fn ; under dependent clause-processor
+    mfc-ts-ttree ; under dependent clause-processor
   ))
 
 (defconst *primitive-macros-with-raw-code*
@@ -34396,6 +34514,125 @@
 ; are likely to be used.
 
                     natp-random$ random$-linear))
+
+; System calls
+
+#-acl2-loop-only
+(defvar *last-sys-call-status* 0)
+
+(defun sys-call (command-string args)
+
+  ":Doc-Section ACL2::ACL2-built-ins
+
+  make a system call to the host operating system~/
+  ~bv[]
+  Example Forms:
+  (sys-call \"cp\" '(\"foo.lisp\" \"foo-copied.lisp\"))
+  (prog2$ (sys-call \"cp\" '(\"foo.lisp\" \"foo-copied.lisp\"))
+          (sys-call-status state))
+  ~ev[]
+  The first argument of ~c[sys-call] is a command for the host operating
+  system, and the second argument is a list of strings that are the
+  arguments for that command.  In GCL and perhaps other lisps, you can put the
+  arguments with the command; but this is not the case, for example, in Allegro
+  CL running on Linux.
+
+  The use of ~ilc[prog2$] above is optional, but illustrates a typical sort
+  of use when one wishes to get the return status.  ~l[sys-call-status].~/
+  ~bv[]
+  General Form:
+  (sys-call cmd args)
+  ~ev[]
+  This function logically returns ~c[nil].  However, it makes the indicated
+  call to the host operating system, as described above, using a function
+  supplied ``under the hood'' by the underlying Lisp system.  On occasions
+  where one wishes to obtain the numeric status returned by the host operating
+  system (or more precisely, by the Lisp function under the hood that passes
+  the system call to the host operating system), one may do so;
+  ~pl[sys-call-status].  The status value is the value returned by that Lisp
+  function, which may well be the same numeric value returned by the host
+  operating system for the underlying system call.
+
+  Note that ~c[sys-call] does not touch the ACL2 ~ilc[state]; however,
+  ~ilc[sys-call-status] updates the ~c[acl2-oracle] field of the ~c[state].
+
+  Be careful if you use ~c[sys-call]!  It can be used for example to overwrite
+  files, or worse!  We view a use of ~c[sys-call] as a call to the operating
+  system that is made outside ACL2.  The following example from Bob Boyer shows
+  how to use ~c[sys-call] to execute, in effect, arbitrary Lisp forms.  ACL2
+  provides a ``trust tag'' mechanism that requires execution of a ~ilc[defttag]
+  form before you can use ~c[sys-call]; ~pl[defttag].  (Note: The setting of
+  the raw Lisp variable ~c[*features*] below is just to illustrate that any
+  such mischief is possible.  Normally ~c[*features*] is a list with more than
+  a few elements.)
+  ~bv[]
+  % cat foo
+  print *0x85d2064=0x838E920
+  detach
+  q
+  % acl2
+  ... boilerplate deleted
+  ACL2 !>(sys-call \"gdb -p $PPID -w < foo >& /dev/null \" nil)
+  NIL
+  ACL2 !>:q
+
+  Exiting the ACL2 read-eval-print loop.  To re-enter, execute (LP).
+  ACL2>*features*
+
+  (:AKCL-SET-MV)
+
+  ACL2>
+  ~ev[]
+
+  Finally, we make a comment about output redirection, which also applies to
+  other related features that one may expect of a shell.  ~c[Sys-call] does not
+  directly support output redirection.  If you want to run a program, ~c[P],
+  and redirect its output, we suggest that you create a wrapper script, ~c[W]
+  to call instead.  Thus ~c[W] might be a shell script containing the line:
+  ~bv[]
+  P $* >& foo.out
+  ~ev[]
+  If this sort of solution proves inadequate, please contact the ACL2
+  implementors and perhaps we can come up with a solution."
+
+  (declare (xargs :guard t))
+  #+acl2-loop-only
+  (declare (ignore command-string args))
+  #-acl2-loop-only 
+  (let ((rslt (system-call command-string args)))
+    (progn (setq *last-sys-call-status* rslt)
+           nil))
+  #+acl2-loop-only
+  nil
+  )
+
+(defun sys-call-status (state)
+
+  ":Doc-Section ACL2::ACL2-built-ins
+
+  exit status from the preceding system call~/
+
+  This function returns two values, ~c[(mv status state)].  The first is the
+  status resulting from the most recent invocation of function ~c[sys-call];
+  ~pl[sys-call].  The second is the ACL2 ~ilc[state] object, which is also the
+  input to this function.~/
+
+  The function ~ilc[sys-call] makes a system call to the host operating system
+  using a function supplied ``under the hood'' by the underlying Lisp system.
+  The status value is the value returned by that Lisp function, which may well
+  be the numeric value returned by the host operating system for the underlying
+  system call.  For more information, ~pl[sys-call].~/"
+
+  (declare (xargs :stobjs state))
+  #-acl2-loop-only
+  (when (live-state-p state)
+    (return-from sys-call-status
+                 (mv *last-sys-call-status* state)))
+  (mv-let (erp val state)
+          (read-acl2-oracle state)
+          (mv (and erp val) state)))
+
+; End of system calls
 
 ; Time:  idate, run-time, and timers.
 
@@ -46124,7 +46361,7 @@ Lisp definition."
   their own hint keywords.  For examples, see the community books directory
   ~c[books/hints/], in particular ~c[basic-tests.lisp].~/~/")
 
-; Start implemenation of search.
+; Start implementation of search.
 
 (defun search-fn-guard (seq1 seq2 from-end test start1 start2 end1 end2
                              end1p end2p)
@@ -48834,3 +49071,438 @@ Lisp definition."
   (let ((form `(set-absstobj-debug-fn ,val ,always)))
     (cond (event-p `(value-triple ,form :on-skip-proofs ,on-skip-proofs))
           (t form))))
+
+; The following functions are defined in logic mode because they will be
+; used in tau bounder correctness theorems.  We basically define two functions,
+; intervalp and in-intervalp, but we also define various subroutines needed to
+; make those functions manageable.  In tau.lisp we define the record structure:
+
+; (defrec tau-interval (domain (lo-rel . lo) . (hi-rel . hi)) t)
+
+; and this is precisely the structure recognized by intervalp and given meaning
+; by in-intervalp.  We therefore achieve the goal that the user can prove
+; theorems about bounder functions defined in terms of the concepts named here
+; and we can run those functions on the actual tau-intervals constructed by the
+; tau system.  (Of course, those actual intervals could have been constructed
+; and accessed by these functions rather than the more efficient record
+; expressions, but efficiency matters.)
+
+; In the guard below, we know when both x and y are non-nil then (at least) one
+; is a rational.  Under that guard, the body below is actually equivalent to the
+; more elegant:
+
+;  (if (or (null x)
+;          (null y))
+;      t
+;      (if rel (< x y) (<= x y)))
+
+; except the body is guard-verifiable while the elegant one is not, since the
+; guard for < (and <=) requires that both arguments be rationals.  This is
+; proved by the thm following the definition.
+
+(defun <? (rel x y)
+  (declare (xargs :guard
+                  (implies (and x y)
+                           (or (real/rationalp x)
+                               (real/rationalp y)))))
+  (if (or (null x) (null y))
+      t
+      (let ((x (fix x))
+            (y (fix y)))
+        (if (real/rationalp x)
+            (if (real/rationalp y)
+                (if rel
+                    (< x y)
+                    (<= x y))
+                (or (< x (realpart y))
+                    (and (= x (realpart y))
+                         (< 0 (imagpart y)))))
+            (or (< (realpart x) y)
+                (and (= (realpart x) y)
+                     (< (imagpart x) 0)))))))
+
+#||
+(thm (implies (implies (and x y)
+                       (or (real/rationalp x)
+                           (real/rationalp y)))
+              (iff (<? rel x y)
+                   (if (or (null x)
+                           (null y))
+                       t
+                       (if rel (< x y) (<= x y)))))
+     :hints
+     (("Goal"
+       :use ((:instance completion-of-< (x x) (y y))
+             (:instance completion-of-< (x y) (y x))))))
+||#
+
+(defun tau-interval-domainp (dom x)
+  (declare (xargs :guard t))
+  (cond ((eq dom 'integerp) (integerp x))
+        ((eq dom 'rationalp) (rationalp x))
+        ((eq dom 'acl2-numberp) (acl2-numberp x))
+; Domain = nil means no restrictions.
+        (t t)))
+
+(defun tau-interval-dom (x)
+  (declare (xargs :guard (consp x)))
+
+  ":Doc-Section tau-system
+
+  access the domain of a tau interval~/
+
+  It is the case that
+  ~bv[]
+  (tau-interval-dom (make-tau-interval dom lo-rel lo hi-rel hi)) = dom
+  ~ev[]
+  ~/
+  For a well-formed interval, ~c[dom] is one of the symbols ~c[INTEGERP],
+  ~c[RATIONALP], ~c[ACL2-NUMBERP], or ~c[NIL].  When the domain is ~c[NIL]
+  there is no domain restriction.
+
+  When the domain is ~c[INTEGERP], there are additional constraints on the
+  other components.  ~l[make-tau-interval].~/"
+
+  (car x))
+
+(defun tau-interval-lo-rel (x)
+  (declare (xargs :guard (and (consp x) (consp (cdr x)) (consp (cadr x)))))
+
+  ":Doc-Section tau-system
+
+  access the lower bound relation of a tau interval~/
+
+  It is the case that
+  ~bv[]
+  (tau-interval-lo-rel (make-tau-interval dom lo-rel lo hi-rel hi)) = lo-rel
+  ~ev[]
+  ~/
+  For a well-formed interval, ~c[lo-rel] is a Boolean, where ~c[t]
+  denotes the ~ilc[<] (strong inequality or ``less-than'') relation and
+  ~c[nil] denotes ~ilc[<=] (weak inequality or ``less-than-or-equal'') relation
+  between the lower bound and the elements of the interval.
+
+  When the domain of an interval is ~c[INTEGERP], there are additional
+  constraints on the other components.  ~l[make-tau-interval].~/"
+
+  (car (cadr x)))
+
+(defun tau-interval-lo (x)
+  (declare (xargs :guard (and (consp x) (consp (cdr x)) (consp (cadr x)))))
+
+  ":Doc-Section tau-system
+
+  access the lower bound of a tau interval~/
+
+  It is the case that
+  ~bv[]
+  (tau-interval-lo (make-tau-interval dom lo-rel lo hi-rel hi)) = lo
+  ~ev[]
+  ~/
+  For a well-formed interval, ~c[lo] is either ~c[nil], denoting negative
+  infinity, or a rational number giving the lower bound of the interval.
+  It must be the case that the lower bound is weakly below the upper bound
+  of a well-formed interval.
+
+  When the domain of an interval is ~c[INTEGERP], there are additional
+  constraints on the other components.  ~l[make-tau-interval].~/"
+
+  (cdr (cadr x)))
+
+(defun tau-interval-hi-rel (x)
+  (declare (xargs :guard (and (consp x) (consp (cdr x)) (consp (cddr x)))))
+  ":Doc-Section tau-system
+
+  access the upper bound relation of a tau interval~/
+
+  It is the case that
+  ~bv[]
+  (tau-interval-hi-rel (make-tau-interval dom lo-rel lo hi-rel hi)) = hi-rel
+  ~ev[]
+  ~/
+  For a well-formed interval, ~c[hi-rel] is a Boolean, where ~c[t]
+  denotes the ~ilc[<] (strong inequality or ``less-than'') relation and
+  ~c[nil] denotes ~ilc[<=] (weak inequality or ``less-than-or-equal'') relation
+  between the elements of the interval and the upper bound.
+
+  When the domain of an interval is ~c[INTEGERP], there are additional
+  constraints on the other components.  ~l[make-tau-interval].~/"
+
+  (car (cddr x)))
+
+(defun tau-interval-hi (x)
+  (declare (xargs :guard (and (consp x) (consp (cdr x)) (consp (cddr x)))))
+
+  ":Doc-Section tau-system
+
+  access the upper bound of a tau interval~/
+
+  It is the case that
+  ~bv[]
+  (tau-interval-hi (make-tau-interval dom lo-rel lo hi-rel hi)) = hi
+  ~ev[]
+  ~/
+  For a well-formed interval, ~c[hi] is either ~c[nil], denoting positive
+  infinity, or a rational number giving the upper bound of the interval.
+  It must be the case that the upper bound is weakly above the lower bound
+  of a well-formed interval.
+
+  When the domain of an interval is ~c[INTEGERP], there are additional
+  constraints on the other components.  ~l[make-tau-interval].~/"
+
+  (cdr (cddr x)))
+
+(defun make-tau-interval (dom lo-rel lo hi-rel hi)
+  (declare (xargs :guard (and (or (null lo) (rationalp lo))
+                              (or (null hi) (rationalp hi)))))
+  ":Doc-Section tau-system
+
+  make a tau interval~/
+
+  ~bv[]
+  General Form:
+  (make-tau-interval doc lo-rel lo hi-rel hi)
+  ~ev[]
+
+  An interval is a structure of the form: ~c[(]~i[dom] ~c[(]~i[lo-rel] ~c[.]
+  ~i[lo]~c[)] ~c[.]  ~c[(]~i[hi-rel] ~c[.] ~i[hi]~c[))].  Every tau contains an
+  interval used to represent the domain, the upper, and the lower bounds of the
+  objects recognized by the tau.~/
+
+  ~c[make-tau-interval] constructs well-formed intervals only if its five arguments
+  satisfy certain restrictions given below.  When these restrictions are
+  violated ~c[make-tau-interval] can construct objects that are not intervals!
+  ~c[make-tau-interval] does not attempt to coerce or adjust its arguments to make
+  well-formed intervals.
+
+  For examples of intervals (and non-intervals!) constructed by
+  ~c[make-tau-interval] see ~ilc[tau-intervalp].  For examples of what objects are
+  contained in certain intervals, see ~ilc[in-tau-intervalp].
+
+  The components of an interval are as follows:
+
+  ~i[dom] (``domain'') -- must be one of four symbols: ~c[INTEGERP],
+  ~c[RATIONALP], ~c[ACL2-NUMBERP], or ~c[NIL] denoting no restriction
+  on the domain.
+
+  The two ``relations,'' ~i[lo-rel] and ~i[hi-rel] are Booleans, where ~c[t]
+  denotes less-than inequality (~ilc[<]) and ~c[nil] represents
+  less-than-or-equal inequality (~ilc[<=]).  Think of ~c[t] meaning ``strong''
+  and ~c[nil] meaning ``weak'' inequality.
+
+  ~i[Lo] and ~i[hi] must be either ~c[nil] or explicit rational numbers.  If
+  ~i[lo] is ~c[nil] it denotes negative infinity; if ~i[hi] is ~c[nil] it
+  denotes positive infinity.  ~i[Lo] must be no greater than ~i[hi].
+  ~i[Note]:  Even though ~c[ACL2-NUMBERP] intervals may contain complex
+  rationals, the ~i[lo] and ~i[hi] bounds must be rational.  This is an
+  arbitrary decision made by the implementors to simplify coding.
+
+  Finally, if the ~i[dom] is ~c[INTEGERP], then both relations should be weak
+  and ~i[lo] and ~i[hi] must be integers when they are non-~c[nil].
+
+  For ~i[x] to be ``in'' an interval it must be of the type described
+  by the domain predicate ~i[dom], ~i[lo] must be smaller than ~i[x] in the
+  strong or weak sense denoted by ~i[lo-rel], and ~i[x] must be smaller than
+  ~i[hi] in the strong or weak sense denoted by ~i[hi-rel].
+
+  The components of an interval may be accessed with the functions
+  ~ilc[tau-interval-dom], ~ilc[tau-interval-lo-rel], ~ilc[tau-interval-lo],
+  ~ilc[tau-interval-hi-rel], and ~ilc[tau-interval-hi].~/"
+
+  (cons dom (cons (cons lo-rel lo)
+                  (cons hi-rel hi))))
+
+(defun tau-intervalp (int)
+  (declare (xargs :guard t))
+
+  ":Doc-Section tau-system
+
+  Boolean recognizer for tau intervals~/
+
+  ~bv[]
+  General Form:
+  (tau-intervalp x)
+  ~ev[]
+  ~/  
+  An interval is a structure of the form: ~c[(]~i[dom] ~c[(]~i[lo-rel] ~c[.]
+  ~i[lo]~c[)] ~c[.]  ~c[(]~i[hi-rel] ~c[.] ~i[hi]~c[))].  Every tau contains an
+  interval used to represent the domain and the upper and lower bounds of the
+  objects recognized by the tau.
+
+  Restrictions on the components of an interval are as follows.  For an
+  interpretation of the meaning of the components, see ~ilc[in-tau-intervalp] or
+  ~ilc[make-tau-interval].
+
+  ~i[dom] (``domain'') -- must be one of four symbols: ~c[INTEGERP],
+  ~c[RATIONALP], ~c[ACL2-NUMBERP], or ~c[NIL].
+
+  The two ``relations,'' ~i[lo-rel] and ~i[hi-rel], must be Booleans.
+
+  ~i[Lo] and ~i[hi] must be either ~c[nil] or explicit rational numbers.
+  ~i[Lo] must be no greater than ~i[hi] (where ~c[nil]s represent negative or
+  positive infinity for ~i[lo] and ~i[hi] respectively.
+
+  Finally, if the ~i[dom] is ~c[INTEGERP], then both relations must ~c[nil]
+  and ~i[lo] and ~i[hi] must be integers when they are non-~c[nil].
+
+  Recall that ~ilc[make-tau-interval] constructs intervals.  The intervals it
+  constructs are well-formed only if the arguments to ~c[make-tau-interval] satisfy
+  the rules above; ~c[make-tau-interval] does not coerce or adjust its
+  arguments in any way.  Thus, it can be (mis-)used to create non-intervals.
+  Here are examples of ~c[tau-intervalp] using ~c[make-tau-interval].
+
+  ~bv[]
+  ; integers: 0 <= x <= 10:
+  (tau-intervalp (make-tau-interval 'INTEGERP nil 0 nil 10))      = t
+
+  ; integers: 0 <= x (i.e., the natural numbers):
+  (tau-intervalp (make-tau-interval 'INTEGERP nil 0 nil nil))     = t
+
+  ; violations of domain rules:
+  (tau-intervalp (make-tau-interval 'INTEGERP t 0 t 10))          = nil
+  (tau-intervalp (make-tau-interval 'INTEGERP nil 0 nil 10/11))   = nil
+
+  ; violation of rule that bounds must be rational if non-nil:
+  (tau-intervalp (make-tau-interval 'ACL2-NUMBERP t 0 t #c(3 5))) = nil
+
+  ; violation of rule that lo <= hi:
+  (tau-intervalp (make-tau-interval 'ACL2-NUMBERP t 0 t -10))     = nil
+
+  ; rationals: 0 < x <= 22/7:
+  (tau-intervalp (make-tau-interval 'RATIONALP t 0 nil 22/7))     = t
+
+  ; numbers: -10 < x < 10:
+  (tau-intervalp (make-tau-interval 'ACL2-NUMBERP t -10 t 10))    = t
+
+  ; any: -10 < x < 10:
+  (tau-intervalp (make-tau-interval nil t -10 t 10))              = t
+
+  : any:
+  (tau-intervalp (make-tau-interval nil nil nil nil nil))         = t
+  ~ev[]
+  Note that the second-to-last interval, with domain ~c[nil] contains all
+  non-numbers as well as numbers strictly between -10 and 10.  The reason is
+  that the interval contains ~c[0] and all non-numbers are coerced to ~c[0] by
+  the inequality functions.
+
+  Note that the last interval contains all ACL2 objects.  It is called the
+  ``universal interval.''~/"
+
+  (if (and (consp int)
+           (consp (cdr int))
+           (consp (cadr int))
+           (consp (cddr int)))
+      (let ((dom (tau-interval-dom int))
+            (lo-rel (tau-interval-lo-rel int))
+            (lo (tau-interval-lo int))
+            (hi-rel (tau-interval-hi-rel int))
+            (hi (tau-interval-hi int)))
+        (cond
+         ((eq dom 'integerp)
+          (and (null lo-rel)
+               (null hi-rel)
+               (if lo
+                   (and (integerp lo)
+                        (if hi
+                            (and (integerp hi)
+                                 (<= lo hi))
+                            t))
+                   (if hi
+                       (integerp hi)
+                       t))))
+         (t (and (member dom '(rationalp acl2-numberp nil))
+                 (booleanp lo-rel)
+                 (booleanp hi-rel)
+                 (if lo
+                     (and (rationalp lo)
+                          (if hi
+                              (and (rationalp hi)
+                                   (<= lo hi))
+                              t))
+                     (if hi
+                         (rationalp hi)
+                         t))))))
+      nil))
+
+(defun in-tau-intervalp (x int)
+  (declare (xargs :guard (tau-intervalp int)))
+
+  ":Doc-Section tau-system
+
+  Boolean membership in a tau interval~/
+
+  ~bv[]
+  General Form:
+  (in-tau-intervalp e x)
+  ~ev[]
+
+  Here, ~c[x] should be an interval (see ~ilc[tau-intervalp]).  This function
+  returns ~c[t] or ~c[nil] indicating whether ~c[e], which is generally but not
+  necessarily a number, is an element of interval ~c[x].  By that is meant that
+  ~c[e] satisfies the domain predicate of the interval and lies between the two
+  bounds.~/
+
+  Suppose ~c[x] is an interval with the components ~i[dom], ~i[lo-rel], ~i[lo],
+  ~i[hi-rel] and ~i[hi].  Suppose ~c[(<? ]~i[rel u v]~c[)] means ~c[(< ]~i[u v]~c[)]
+  when ~i[rel] is true and ~c[(<= ]~i[u v]~c[)] otherwise, with appropriate
+  treatment of infinities.
+
+  Then for ~c[e] to be in interval ~c[x], it must be the case that ~c[e]
+  satisfies the domain predicate ~i[dom] (where where ~i[dom]=~c[nil] means
+  there is no restriction on the domain) and ~c[(<? ]~i[lo-rel lo]~c[ e)] and
+  ~c[(<? ]~i[hi-rel]~c[ e ]~i[hi]~c[)].  [Note:  ``Appropriate treatment of
+  infinities'' is slightly awkward if both infinities are represented by the
+  same object, ~c[nil].  However, this is handled by coercing ~c[e] to a
+  number ~i[after] checking that it is in the domain.  By this trick, ``~c[<?]''
+  is presented with at most one ``infinity'' and it is always negative
+  when in the first argument and positive when in the second.]
+
+  Note that every element in an ~c[INTEGERP] interval is contained in the
+  analogous ~c[RATIONALP] interval (i.e., the interval obtained by just
+  replacing the domain ~c[INTEGERP] by ~c[RATIONALP]).  That is because every
+  integer is a rational.  Similarly, every rational is an ACL2 number.
+
+  Note that an interval in which the relations are weak and the bounds are
+  equal rationals is the ``unit'' or ``identity'' interval containing exactly
+  that rational.
+
+  Note that an interval in which the relations are strong and the bounds are
+  equal rationals is empty:  it contains no objects.
+
+  Note that the interval ~c[(make-tau-interval nil nil nil nil nil)] is the
+  ``universal interval:'' it contains all ACL2 objects.  It contains all
+  numbers because they statisfy the non-existent domain restriction and lie
+  between minus infinity and plus infinity.  It contains all non-numbers
+  because the interval contains ~c[0] and ACL2's inequalities coerce
+  non-numbers to ~c[0].  The universal interval is useful if you are defining a
+  bounder (~pl[bounders]) for a function and do not wish to address a certain
+  case: return the universal interval.
+
+  Recall that ~ilc[make-tau-interval] constructs intervals.  Using ~c[make-tau-interval]
+  we give several self-explanatory examples of ~c[in-tau-intervalp]:
+
+  ~bv[]
+  (in-tau-intervalp 3 (make-tau-interval 'INTEGERP nil 0 nil 10))           = t
+  (in-tau-intervalp 3 (make-tau-interval 'RATIONALP nil 0 nil 10))          = t
+  (in-tau-intervalp 3 (make-tau-interval NIL nil 0 nil 10))                 = t
+
+  (in-tau-intervalp -3 (make-tau-interval 'INTEGERP nil 0 nil 10))          = nil
+  (in-tau-intervalp 30 (make-tau-interval 'INTEGERP nil 0 nil 10))          = nil
+
+  (in-tau-intervalp 3/5 (make-tau-interval 'INTEGERP nil 0 nil 10))         = nil
+  (in-tau-intervalp 3/5 (make-tau-interval 'RATIONALP nil 0 nil 10))        = t
+
+  (in-tau-intervalp #c(3 5) (make-tau-interval 'RATIONALP nil 0 nil 10))    = nil
+  (in-tau-intervalp #c(3 5) (make-tau-interval 'ACL2-NUMBERP nil 0 nil 10)) = t
+
+  (in-tau-intervalp 'ABC (make-tau-interval NIL nil 0 nil 10))               = t
+  ~ev[]
+  ~/"
+
+  (and (tau-interval-domainp (tau-interval-dom int) x)
+       (<? (tau-interval-lo-rel int)
+           (tau-interval-lo int)
+           (fix x))
+       (<? (tau-interval-hi-rel int)
+           (fix x)
+           (tau-interval-hi int))))
